CSwL.lean
@@ -1,4 +1,3 @@
-import CSwL.Chapter01
 import CSwL.Chapter02
 import CSwL.Chapter03
 import CSwL.Chapter04
